UnitTest/AttrParser.lean
@@ -60,7 +60,7 @@ macro "#assert " e:term : command =>
 
 #assert expectError "\"" "expected '\"' in string literal"
 
-#assert expectSuccess "i32" (integerType 32).asType
-#assert expectSuccess "i0" (integerType 0).asType
+#assert expectSuccess "i32" IntegerType.mk 32
+#assert expectSuccess "i0" IntegerType.mk 0
 #assert expectMissing "foo"
 #assert expectMissing "i0x4"
